{
 "cells": [
  {
   "cell_type": "markdown",
   "metadata": {},
   "source": [
    "# Hermite Interpolation\n",
    "\n",
    "To improve the interpolation accuracy without increasing the number of interpolation nodes, one feasible way is to take derivative values into consideration. That is to say, the interplant should satisfies:\n",
    "\n",
    "$$\n",
    "\\begin{cases}\n",
    "    H_n(x_i) = y_i \\\\\n",
    "    H_n'(x_i) = y'_i\n",
    "\\end{cases}\n",
    "$$\n",
    "\n",
    "Based on the idea of **Lagrange Interpolation**, the form of **Hermite Interpolant** can be set as:\n",
    "\n",
    "$$\n",
    "H_{2n+1}(x) = \\sum_{j=0}^n \\alpha_j(x)y_j + \\sum_{j=0}^n \\beta_j(x)y'_j\n",
    "$$\n",
    "\n",
    "The first **basis polynomial** $\\alpha_j(x)$ meets the condition below:\n",
    "\n",
    "$$\n",
    "\\begin{array}{ccc}\n",
    "    \\text{label} & \\text{x} & \\text{y} & \\text{y'} \\\\\n",
    "    \\hline\n",
    "    0 & x_0 & 0 & 0 \\\\\n",
    "    \\hline\n",
    "    1 & x_1 & 0 & 0 \\\\\n",
    "    \\hline\n",
    "    2 & x_2 & 0 & 0 \\\\\n",
    "    \\hline\n",
    "    ... & ... & ... & ... \\\\\n",
    "    \\hline\n",
    "    j & x_j & 1 & 0 \\\\\n",
    "    \\hline\n",
    "    ... & ... & ... & ... \\\\\n",
    "    \\hline\n",
    "    n & x_n & 0 & 0 \\\\\n",
    "    \\hline\n",
    "\\end{array}\n",
    "$$\n",
    "\n",
    "In other words, all $x$ s except $x_j$ are dual roots of $\\alpha_j(x)$. So we can set $\\alpha_j(x)$ in the form of:\n",
    "$$\n",
    "\\alpha_j(x) = (ax+b)\\cdot l^2_j(x),\n",
    "$$\n",
    "\n",
    "where $l_j(x)$ is the basis polynomial of **Lagrange Interpolation**.\n",
    "\n",
    "With conditions:\n",
    "\n",
    "$$\n",
    "\\begin{cases}\n",
    "    \\alpha_j(x_j) = ax_j + b = 1 \\\\\n",
    "    \\alpha_j'(x_j) = a + 2(ax_j + b)\\cdot l'_j(x_j) = 0\n",
    "\\end{cases}\n",
    "$$\n",
    "\n",
    "We can get:\n",
    "\n",
    "$$\n",
    "\\alpha_j(x) = [1+2l'_j(x_j)(x_j - x)]\\cdot l^2_j(x)\n",
    "$$\n",
    "\n",
    "In this expression, $l'_j(x_j)$ is calculated by:\n",
    "\n",
    "$$\n",
    "l'_j(x_j) = l_j(x_j) \\prod_{i=0, i \\neq j}^n \\frac{1}{x-x_i} = \\prod_{i=0, i \\neq j}^n \\frac{1}{x-x_i}\n",
    "$$\n",
    "\n",
    "As for the second **basis polynomial** $\\beta_j(x)$, it meets the conition below:\n",
    "\n",
    "$$\n",
    "\\begin{array}{ccc}\n",
    "    \\text{label} & \\text{x} & \\text{y} & \\text{y'} \\\\\n",
    "    \\hline\n",
    "    0 & x_0 & 0 & 0 \\\\\n",
    "    \\hline\n",
    "    1 & x_1 & 0 & 0 \\\\\n",
    "    \\hline\n",
    "    2 & x_2 & 0 & 0 \\\\\n",
    "    \\hline\n",
    "    ... & ... & ... & ... \\\\\n",
    "    \\hline\n",
    "    j & x_j & 0 & 1 \\\\\n",
    "    \\hline\n",
    "    ... & ... & ... & ... \\\\\n",
    "    \\hline\n",
    "    n & x_n & 0 & 0 \\\\\n",
    "    \\hline\n",
    "\\end{array}\n",
    "$$\n",
    "\n",
    "We can also set $\\beta_j(x)$ in the form of:\n",
    "\n",
    "$$\n",
    "\\beta_j(x) = (Ax+B)l^2_j(x)\n",
    "$$\n",
    "\n",
    "With conditions:\n",
    "\n",
    "$$\n",
    "\\begin{cases}\n",
    "    \\beta_j(x_j) = Ax_j + B = 0 \\\\\n",
    "    \\beta_j'(x_j) = A + 2(Ax_j + B)\\cdot l'_j(x_j) = 1\n",
    "\\end{cases}\n",
    "$$\n",
    "\n",
    "We can get:\n",
    "\n",
    "$$\n",
    "\\beta_j(x) = (x-x_j)\\cdot l^2_j(x)\n",
    "$$\n",
    "\n",
    "Together, the **Hermite Interpolant** is finalized:\n",
    "\n",
    "$$\n",
    "H_{2n+1}(x) = \\sum_{j=0}^n [y_j + (x-x_j)(y'_j - 2y_jl'_j(x_j))]\\cdot l^2_j(x)\n",
    "$$"
   ]
  },
  {
   "cell_type": "code",
   "execution_count": 3,
   "metadata": {},
   "outputs": [
    {
     "name": "stdout",
     "output_type": "stream",
     "text": [
      "Estimated y is: [0.81613106 1.08278184]\n",
      "Error is: [2.00099664e-08 1.85818658e-08]\n"
     ]
    }
   ],
   "source": [
    "import numpy as np\n",
    "\n",
    "def hermite_interpolation(func, func_diff, X, x_interp):\n",
    "    n = len(X)\n",
    "    Y = np.zeros(n)\n",
    "    Y_diff = np.zeros(n)\n",
    "    y = np.zeros(len(x_interp))\n",
    "    \n",
    "    for i in range(n):\n",
    "        Y[i] = func(X[i])\n",
    "        Y_diff[i] = func_diff(X[i])\n",
    "        \n",
    "    for k in range(len(x_interp)):\n",
    "        x_k = x_interp[k]\n",
    "        y_k = 0\n",
    "        \n",
    "        for i in range(n):\n",
    "            Li = 1\n",
    "            Li_diff = 0\n",
    "            \n",
    "            for j in range(n):\n",
    "                if j != i:\n",
    "                    Li = Li * ((x_k - X[j]) / (X[i] - X[j]))\n",
    "                    Li_diff = Li_diff + 1 / (X[i] - X[j])\n",
    "                    \n",
    "            y_k = y_k + Li**2 * (Y[i] + (x_k - X[i]) * (Y_diff[i] - 2 * Y[i] * Li_diff))\n",
    "        \n",
    "        y[k] = y_k\n",
    "        \n",
    "    err = np.zeros(len(x_interp))\n",
    "    y_acc = np.zeros(len(x_interp))\n",
    "    for i in range(len(x_interp)):\n",
    "        y_acc[i] = func(x_interp[i])\n",
    "        err[i] = abs(y_acc[i] - y[i])\n",
    "        \n",
    "    print(f\"Estimated y is: {y}\")\n",
    "    print(f\"Error is: {err}\")\n",
    "    \n",
    "def func(x):\n",
    "    return x * np.log(1+x)\n",
    "\n",
    "def func_diff(x):\n",
    "    return np.log(1+x) + x / (1+x)\n",
    "\n",
    "X = np.array([1,1.2,1.4])\n",
    "x_interp = np.array([1.1,1.3])\n",
    "hermite_interpolation(func, func_diff, X, x_interp)"
   ]
  }
 ],
 "metadata": {
  "kernelspec": {
   "display_name": "edward",
   "language": "python",
   "name": "edward"
  },
  "language_info": {
   "codemirror_mode": {
    "name": "ipython",
    "version": 3
   },
   "file_extension": ".py",
   "mimetype": "text/x-python",
   "name": "python",
   "nbconvert_exporter": "python",
   "pygments_lexer": "ipython3",
   "version": "3.12.5"
  }
 },
 "nbformat": 4,
 "nbformat_minor": 2
}
